tests/lean/run/5407.lean
@@ -1,0 +1,86 @@
+/-!
+# Library search should not return invalid tactics
+
+https://github.com/leanprover/lean4/issues/5407
+
+The library-search tactics `exact?` and `apply?` should not suggest proof terms that do not
+compile. If such proof terms are generated, these tactics should instead provide users with
+appropriate feedback.
+-/
+
+/-! Discards unprintable implicit argument to lambda -/
+inductive Odd : Nat → Prop
+  | one : Odd 1
+  | add_two : Odd n → Odd (n + 2)
+
+theorem odd_iff {n : Nat} : Odd n ↔ n % 2 = 1 := by
+  refine ⟨fun h => by induction h <;> omega, ?_⟩
+  match n with
+  | 0 => simp
+  | 1 => exact fun _ => Odd.one
+  | n + 2 => exact fun _ => Odd.add_two (odd_iff.mpr (by omega))
+
+/--
+error: found a proof, but the corresponding tactic
+  exact fun a => (fun {n} => odd_iff.mpr) a
+aborted unexpectedly
+-/
+#guard_msgs in
+example {n : Nat} : n % 2 = 1 → Odd n :=
+  by exact?
+
+
+/-! Detects shadowed variables -/
+opaque A : Type
+opaque B : Type
+opaque C : Prop
+theorem imp : A → B → C := sorry
+/--
+error: found a proof, but the corresponding tactic
+  exact imp h✝ h
+is invalid because the following variables have inaccessible names:
+  h✝
+To fix this, ensure these variables are not shadowed and are given explicit names when introduced.
+-/
+#guard_msgs in
+example : C := by
+  have h : A := sorry
+  have h : B := sorry
+  exact?
+
+
+/-! Detects lambdas with insufficient explicit binder types -/
+inductive EqExplicit {α} : α → α → Prop
+  | intro : (a b : α) → a = b → EqExplicit a b
+/--
+error: found a proof, but the corresponding tactic
+  exact EqExplicit.intro (fun f => (fun g x => g x) f) id rfl
+failed with the following error:
+  application type mismatch
+    EqExplicit.intro (fun f => (fun g x => ?m.5093) f) ?m.5146 rfl
+  argument
+    rfl
+  has type
+    ?m.5160 = ?m.5160 : Prop
+  but is expected to have type
+    (fun f => (fun g x => ?m.5093) f) = ?m.5146 : Prop
+-/
+#guard_msgs in
+example : EqExplicit (fun (f : α → β) => (fun g x => g x) f) id := by
+  exact?
+
+/-! `apply?` logs info instead of erroring -/
+opaque D : Prop
+theorem option1 : A → D := sorry
+theorem option2 {_ : B} :  D := sorry
+/--
+info: Try this: refine option1 ?_
+---
+info: found a partial proof, but the corresponding tactic
+  refine option2
+aborted unexpectedly
+---
+warning: declaration uses 'sorry'
+-/
+#guard_msgs in
+example : D := by apply?
